ulib/FStar.Custard.fst
@@ -1,0 +1,6 @@
+module FStar.Custard
+
+let no_specialize : unit = ()
+
+[@@ no_specialize]
+let dyn (#a:Type) (x:a) : Pure a (requires True) (ensures fun r -> r == x) = x
